fits_stack proofs reveal bug in frame size calculation

compiler/src/compiler/FitsStack.v
@@ -12,27 +12,41 @@ Local Open Scope Z_scope.
 Section FitsStack.
   Context {p: FlatToRiscvCommon.parameters}.
 
-  Definition stack_usage_impl(outer_rec: env -> stmt Z -> option Z)(e: env): stmt Z -> option Z :=
+  (* returns two numbers:
+     - number of stack words needed by current statement
+     - number of stack words needed by its callees
+     The total required stack is the sum of the two. *)
+  Definition stack_usage_impl(outer_rec: env -> stmt Z -> option (Z*Z))(e: env): stmt Z -> option (Z*Z) :=
     fix inner_rec s :=
       match s with
-      | SLoad _ _ _ | SStore _ _ _ | SLit _ _ | SOp _ _ _ _ | SSet _ _ | SSkip | SInteract _ _ _ => Some 0
+      | SLoad _ _ _ | SStore _ _ _ | SLit _ _ | SOp _ _ _ _ | SSet _ _ | SSkip | SInteract _ _ _ => Some (0,0)
+      | SStackalloc x n body =>
+        if Z.leb 0 n then
+          if Z.eqb (n mod SeparationLogic.bytes_per_word) 0 then
+            match inner_rec body with
+            | Some (M, N) => Some (M + n / SeparationLogic.bytes_per_word, N)
+            | None => None
+            end
+          else None
+        else None
       | SIf _ s1 s2 | SLoop s1 _ s2 | SSeq s1 s2 =>
         match inner_rec s1, inner_rec s2 with
-        | Some u1, Some u2 => Some (Z.max u1 u2)
+        | Some (M1, N1), Some (M2, N2) => Some (Z.max M1 M2, Z.max N1 N2)
         | _, _ => None
         end
       | SCall binds fname args =>
         match map.get e fname with
         | Some (argnames, retnames, body) =>
           match outer_rec (map.remove e fname) body with
-          | Some u => Some (framelength (argnames, retnames, body) + u)
+          (* M is already accounted for in framelength *)
+          | Some (M, N) => Some (0, N + framelength (argnames, retnames, body))
           | None => None
           end
         | None => None
         end
     end.
 
-  Fixpoint stack_usage_rec(env_size_S: nat): env -> stmt Z -> option Z :=
+  Fixpoint stack_usage_rec(env_size_S: nat): env -> stmt Z -> option (Z*Z) :=
     match env_size_S with
     | O => fun _ _ => None
     | S env_size => stack_usage_impl (stack_usage_rec env_size)
@@ -43,7 +57,10 @@ Section FitsStack.
   (* returns the number of stack words needed to execute f_entrypoint (which must have no args
      and no return values), None if a function not in funimpls is called or a function is recursive *)
   Definition stack_usage_of_fun(funimpls: env)(f_entrypoint: String.string): option Z :=
-    stack_usage_rec (S (count_funs funimpls)) funimpls (SCall nil f_entrypoint nil).
+    match stack_usage_rec (S (count_funs funimpls)) funimpls (SCall nil f_entrypoint nil) with
+    | Some (M, N) => Some (M + N)
+    | None => None
+    end.
 
   Definition update_stack_usage(e_glob: env)
              (current: option Z)(fname: String.string)(fimpl: list Z * list Z * stmt Z): option Z :=
@@ -61,17 +78,16 @@ Section FitsStack.
   Definition stack_usage(funimpls: env): option Z :=
     map.fold (update_stack_usage funimpls) (Some 0) funimpls.
 
-  Lemma fits_stack_monotone: forall e z1 s,
-      fits_stack z1 e s -> forall z2, z1 <= z2 -> fits_stack z2 e s.
+  Lemma fits_stack_monotone: forall e y1 z1 s,
+      fits_stack y1 z1 e s -> forall y2 z2, y1 <= y2 -> z1 <= z2 -> fits_stack y2 z2 e s.
   Proof.
-    induction 1; intros; econstructor; eauto; try blia.
-    eapply IHfits_stack. blia.
+    induction 1; intros; econstructor; eauto; try blia; eapply IHfits_stack; blia.
   Qed.
 
   Context {env_ok: map.ok env}.
 
-  Lemma fits_stack_monotone_env: forall e1 z s,
-      fits_stack z e1 s -> forall e2, map.extends e2 e1 -> fits_stack z e2 s.
+  Lemma fits_stack_monotone_env: forall e1 y z s,
+      fits_stack y z e1 s -> forall e2, map.extends e2 e1 -> fits_stack y z e2 s.
   Proof.
     induction 1; intros; econstructor; eauto; try blia.
     eapply IHfits_stack. (* TODO make map solver work: Solver.map_solver env_ok. *)
@@ -79,23 +95,76 @@ Section FitsStack.
     intros.
     rewrite map.get_remove_dec.
     Tactics.destruct_one_match.
-    - subst. rewrite map.get_remove_same in H2. assumption.
-    - rewrite map.get_remove_diff in H2 by congruence. eauto.
+    - subst. rewrite map.get_remove_same in H3. assumption.
+    - rewrite map.get_remove_diff in H3 by congruence. eauto.
   Qed.
 
-  Lemma stack_usage_rec_correct: forall n e s z,
-      stack_usage_rec n e s = Some z ->
-      fits_stack z e s.
+  Lemma stack_usage_rec_equals_stackalloc_words: forall n s e M N,
+      stack_usage_rec n e s = Some (M, N) ->
+      M = FlatToRiscvDef.stackalloc_words s.
+  Proof.
+    induction n; intros; simpl in *. 1: discriminate.
+    revert M N H.
+    induction s; intros; simpl in *; simp;
+      try specialize IHs with (1 := eq_refl);
+      try specialize IHs1 with (1 := eq_refl);
+      try specialize IHs2 with (1 := eq_refl);
+      try blia.
+    subst.
+    apply Z.leb_le in E. apply Z.eqb_eq in E0.
+    assert (0 < SeparationLogic.bytes_per_word). {
+      unfold SeparationLogic.bytes_per_word.
+      destruct Utility.width_cases as [F|F]; rewrite F; reflexivity.
+    }
+    assert (0 <= nbytes / SeparationLogic.bytes_per_word). {
+      apply Z.div_pos; assumption.
+    }
+    remember (FlatToRiscvDef.stackalloc_words s) as sw.
+    remember (SeparationLogic.bytes_per_word) as bw.
+    (* TODO why does "Z.div_mod_to_equations. blia." not work? *)
+    replace (BinIntDef.Z.max 0 nbytes) with nbytes by blia.
+    apply Zmod_divides in E0. 2: blia.
+    simp.
+    replace (bw * c + bw - 1) with (c * bw + (bw - 1)) by blia.
+    rewrite Z.div_add_l by blia.
+    rewrite (Z.div_small (bw - 1) bw) by blia.
+    rewrite Z.mul_comm.
+    rewrite Z.div_mul; blia.
+  Qed.
+
+  Lemma stack_usage_rec_correct: forall n e s y z,
+      stack_usage_rec n e s = Some (y, z) ->
+      fits_stack y z e s.
   Proof.
     induction n; intros.
     - simpl in H. discriminate.
     - simpl in H.
-      revert z H.
+      revert y z H.
       induction s; intros; simpl in H; simp.
       all: try (constructor; eauto using fits_stack_monotone, Z.le_max_l, Z.le_max_r; blia).
-      econstructor. 1: eassumption.
-      eapply IHn. Fail rewrite E0. (* PARAMRECORDS *) etransitivity. 1: exact E0.
-      f_equal. unfold framelength. blia.
+      + specialize (IHs _ _ eq_refl).
+        pose proof fits_stack_nonneg as P. specialize P with (1 := IHs).
+        apply Z.leb_le in E. apply Z.eqb_eq in E0.
+        econstructor.
+        * assert (0 <= nbytes / SeparationLogic.bytes_per_word). {
+            apply Z.div_pos. 1: assumption. unfold SeparationLogic.bytes_per_word.
+            destruct Utility.width_cases as [F|F]; rewrite F; reflexivity.
+          }
+          blia.
+        * assumption.
+        * assumption.
+        * rewrite Z.add_simpl_r. assumption.
+      + specialize IHn with (1 := E0).
+        pose proof fits_stack_nonneg as P. specialize P with (1 := IHn). destruct P.
+        econstructor. 1: reflexivity. 1: eassumption.
+        pose proof stack_usage_rec_equals_stackalloc_words as P.
+        specialize P with (1 := E0). subst.
+        match goal with
+        | |- fits_stack _ ?z _ _ => replace z with z1
+        end.
+        1: assumption.
+        unfold framelength.
+        blia.
   Qed.
 
   (* The art of figuring out the right induction hypothesis... *)
@@ -104,7 +173,8 @@ Section FitsStack.
       r = Some z ->
       map.get e_done f = Some (nil, nil, fbody) ->
       map.split e_glob e_done e_rest ->
-      fits_stack (z - framelength (nil, nil, fbody)) (map.remove e_glob f) fbody.
+      fits_stack (FlatToRiscvDef.stackalloc_words fbody)
+                 (z - framelength (nil, nil, fbody)) (map.remove e_glob f) fbody.
 
   Lemma stack_usage_correct_aux: forall e_glob e_done,
       P e_glob e_done (map.fold (update_stack_usage e_glob) (Some 0) e_done).
@@ -123,12 +193,12 @@ Section FitsStack.
         simpl in H1.
         simp.
         assert (map.get e_glob k = Some (nil, nil, newbody)) as Q. {
-          clear -H3 E0 H env_ok.
+          clear -H3 E1 H env_ok.
           unfold map.split, map.disjoint in *.
           simp.
-          etransitivity. 1: exact E0.
-          rewrite map.get_putmany_left in E0.
-          - rewrite map.get_put_same in E0. congruence.
+          etransitivity. 1: exact E1.
+          rewrite map.get_putmany_left in E1.
+          - rewrite map.get_put_same in E1. congruence.
           - match goal with
             | |- ?x = None => destr x
             end.
@@ -137,18 +207,21 @@ Section FitsStack.
             eapply H3r. 2: exact E.
             rewrite map.get_put_same. reflexivity.
         }
-        simpl in Q,E0. rewrite Q in E0. symmetry in E0. simp.
+        simpl in Q,E1. rewrite Q in E1. symmetry in E1. simp.
         rewrite map.get_put_dec in H2.
-        eapply stack_usage_rec_correct in E1.
+        pose proof stack_usage_rec_equals_stackalloc_words as P.
+        specialize P with (1 := E2). subst.
+        eapply stack_usage_rec_correct in E2.
         destr (String.eqb k f).
         * simp. subst.
           eapply fits_stack_monotone. 1: eassumption.
-          unfold framelength.
-          blia.
+          all: unfold framelength.
+          all: blia.
         * specialize H0 with (1 := eq_refl).
           eapply fits_stack_monotone.
           -- eauto.
           -- blia.
+          -- unfold framelength. blia.
       }
       all: rewrite map.get_put_dec in H2.
       all: destr (String.eqb k f); try discriminate.
@@ -158,7 +231,8 @@ Section FitsStack.
   Lemma stack_usage_correct: forall e z f fbody,
       map.get e f = Some (nil, nil, fbody) ->
       stack_usage e = Some z ->
-      fits_stack (z - framelength (nil, nil, fbody)) (map.remove e f) fbody.
+      fits_stack (FlatToRiscvDef.stackalloc_words fbody)
+                 (z - framelength (nil, nil, fbody)) (map.remove e f) fbody.
   Proof.
     intros. unfold stack_usage in *.
     pose proof stack_usage_correct_aux as Q.
